small step implies big step

LeanIMP/SmallStepBasic.lean
@@ -22,26 +22,26 @@ inductive SmallStep {α: Type} [BEq α] : IMPProgram α → IMPState α → IMPS
   | ss_if_false (b_expr : BoolExpr α) (p_then p_else : IMPProgram α) (s : IMPState α) :
     (evalBoolExpr b_expr).run s = (false, s) ->
     SmallStep (IMPProgram.«if» b_expr p_then p_else) s (IMPSmallStepState.ss_unfinished p_else s)
-  | ss_while (b_expr : BoolExpr α) (p_body : IMPProgram α) (s s1 : IMPState α) :
+  | ss_while (b_expr : BoolExpr α) (p_body : IMPProgram α) (s : IMPState α) :
     SmallStep (IMPProgram.«while» b_expr p_body) s (
       IMPSmallStepState.ss_unfinished (
         (IMPProgram.«if» b_expr (
           IMPProgram.seq (p_body) (IMPProgram.«while» b_expr p_body)
         ) IMPProgram.skip)
       )
-      s1
+      s
     )
 
 notation "⟨" p:1 "," s:0 "⟩" " ->1 " s':0 => SmallStep p s (IMPSmallStepState.ss_finished s')
 notation "⟨" p:1 "," s:0 "⟩" " ->1 " "⟨" p':1 "," s':0 "⟩" => SmallStep p s (IMPSmallStepState.ss_unfinished p' s')
 
-inductive SmallStepSequence {α: Type} [BEq α] : IMPProgram α → IMPState α → IMPState α → Prop where
+inductive SmallStepSequence {α: Type} [BEq α] : IMPProgram α → IMPState α → IMPState α → Nat -> Prop where
   | single (p: IMPProgram α) (s s': IMPState α) :
     SmallStep p s (IMPSmallStepState.ss_finished s') ->
-    SmallStepSequence p s s'
-  | cons (p1 p2: IMPProgram α) (s s' s'': IMPState α) :
+    SmallStepSequence p s s' 1
+  | cons (p1 p2: IMPProgram α) (s s' s'': IMPState α) (k: Nat) :
     SmallStep p1 s (IMPSmallStepState.ss_unfinished p2 s') ->
-    SmallStepSequence p2 s' s'' ->
-    SmallStepSequence p1 s s''
+    SmallStepSequence p2 s' s'' k ->
+    SmallStepSequence p1 s s'' (1 + k)
 
-notation "⟨" p:1 "," s:0 "⟩" " ->* " s':0 => SmallStepSequence p s s'
+notation "⟨" p:1 "," s:0 "⟩" " ->*" " [" n "] " s':0 => SmallStepSequence p s s' n
