LeanIMP/Equivalence.lean
@@ -6,29 +6,152 @@ import LeanIMP.SmallStep
 
 theorem big_step_implies_small_step {α: Type} [BEq α] {p: IMPProgram α} {s s': IMPState α}
   (big_step : BigStep p s s') :
-  SmallStepSequence p s s' :=
+  ∃k: Nat, SmallStepSequence p s s' k :=
   by
     induction big_step with
-    | bs_skip s => exact SmallStepSequence.single IMPProgram.skip s s (SmallStep.ss_skip s)
-    | bs_assign x e s val eval => exact SmallStepSequence.single (IMPProgram.assign x e) s (s.update x val) (SmallStep.ss_assign x e s val eval)
+    | bs_skip s =>
+      exists 1
+      exact SmallStepSequence.single IMPProgram.skip s s (SmallStep.ss_skip s)
+    | bs_assign x e s val eval =>
+      exists 1
+      exact SmallStepSequence.single (IMPProgram.assign x e) s (s.update x val) (SmallStep.ss_assign x e s val eval)
     | bs_seq p1 p2 s s1 s2 p1_ass p2_ass p1_ih p2_ih =>
+      let ⟨k1, p1_ih⟩ := p1_ih
+      let ⟨k2, p2_ih⟩ := p2_ih
+      exists (k1 + k2)
       exact small_step_sequence_composeable p1_ih p2_ih
     | bs_if_true b_expr p_then p_else s s' eval p_then_tree p_then_ih =>
       have if_step := SmallStep.ss_if_true b_expr p_then p_else s eval
-      exact SmallStepSequence.cons (IMPProgram.«if» b_expr p_then p_else) p_then s s s' if_step p_then_ih
+      let ⟨k1, p_then_ih⟩ := p_then_ih
+      exists (1 + k1)
+      exact SmallStepSequence.cons (IMPProgram.«if» b_expr p_then p_else) p_then s s s' k1 if_step p_then_ih
     | bs_if_false b_expr p_then p_else s s' eval p_then_tree p_else_ih =>
       have if_step := SmallStep.ss_if_false b_expr p_then p_else s eval
-      exact SmallStepSequence.cons (IMPProgram.«if» b_expr p_then p_else) p_else s s s' if_step p_else_ih
+      let ⟨k1, p_else_ih⟩ := p_else_ih
+      exists (1 + k1)
+      exact SmallStepSequence.cons (IMPProgram.«if» b_expr p_then p_else) p_else s s s' k1 if_step p_else_ih
     | bs_while_true b_expr p_body s s1 s2 eval p_body_tree while_continues_tree p_body_ih while_continues_ih =>
-      refine SmallStepSequence.cons (IMPProgram.«while» b_expr p_body) (IMPProgram.«if» b_expr (IMPProgram.seq (p_body) (IMPProgram.«while» b_expr p_body)) IMPProgram.skip) s s s2 ?_ ?_
-      exact SmallStep.ss_while b_expr p_body s s
-      refine SmallStepSequence.cons (IMPProgram.«if» b_expr (IMPProgram.seq (p_body) (IMPProgram.«while» b_expr p_body)) IMPProgram.skip) (IMPProgram.seq (p_body) (IMPProgram.«while» b_expr p_body)) s s s2 ?_ ?_
+      let ⟨k_body, p_body_ih⟩ := p_body_ih
+      let ⟨k_continues, while_continues_ih⟩ := while_continues_ih
+      refine ⟨(1 + (1 + (k_body + k_continues))), SmallStepSequence.cons (IMPProgram.«while» b_expr p_body) (IMPProgram.«if» b_expr (IMPProgram.seq (p_body) (IMPProgram.«while» b_expr p_body)) IMPProgram.skip) s s s2 (1 + (k_body + k_continues)) ?_ ?_⟩
+      exact SmallStep.ss_while b_expr p_body s
+      refine SmallStepSequence.cons (IMPProgram.«if» b_expr (IMPProgram.seq (p_body) (IMPProgram.«while» b_expr p_body)) IMPProgram.skip) (IMPProgram.seq (p_body) (IMPProgram.«while» b_expr p_body)) s s s2 (k_body + k_continues) ?_ ?_
       exact SmallStep.ss_if_true b_expr (IMPProgram.seq (p_body) (IMPProgram.«while» b_expr p_body)) (IMPProgram.skip) s eval
       refine small_step_sequence_composeable ?_ while_continues_ih
       exact p_body_ih
     | bs_while_false b_expr p_body s eval =>
-      refine SmallStepSequence.cons (IMPProgram.«while» b_expr p_body) (IMPProgram.«if» b_expr (IMPProgram.seq (p_body) (IMPProgram.«while» b_expr p_body)) IMPProgram.skip) s s s ?_ ?_
-      exact SmallStep.ss_while b_expr p_body s s
-      refine SmallStepSequence.cons (IMPProgram.«if» b_expr (IMPProgram.seq (p_body) (IMPProgram.«while» b_expr p_body)) IMPProgram.skip) (IMPProgram.skip) s s s ?_ ?_
+      exists 3
+      refine SmallStepSequence.cons (IMPProgram.«while» b_expr p_body) (IMPProgram.«if» b_expr (IMPProgram.seq (p_body) (IMPProgram.«while» b_expr p_body)) IMPProgram.skip) s s s 2 ?_ ?_
+      exact SmallStep.ss_while b_expr p_body s
+      refine SmallStepSequence.cons (IMPProgram.«if» b_expr (IMPProgram.seq (p_body) (IMPProgram.«while» b_expr p_body)) IMPProgram.skip) (IMPProgram.skip) s s s 1 ?_ ?_
       exact SmallStep.ss_if_false b_expr (IMPProgram.seq (p_body) (IMPProgram.«while» b_expr p_body)) IMPProgram.skip s eval
       exact SmallStepSequence.single IMPProgram.skip s s (SmallStep.ss_skip s)
+
+
+
+
+
+theorem small_step_implies_big_step {α: Type} [BEq α] :
+  ∀k: Nat, ∀p: IMPProgram α, ∀s s': IMPState α, SmallStepSequence p s s' k ->
+  BigStep p s s' :=
+  by
+    intros k
+    refine strong_induction_on (fun x => ∀p: IMPProgram α, ∀s s': IMPState α, SmallStepSequence p s s' x -> BigStep p s s') k ?_
+    simp
+    intros n
+    intros ih
+    intros p
+    intros s s'
+    intros small_step
+    let small_step2 := small_step
+    cases small_step with
+      | single p s s' tree =>
+        match tree with
+          | SmallStep.ss_skip s => exact BigStep.bs_skip s
+          | SmallStep.ss_assign x e s val eval => exact BigStep.bs_assign x e s val eval
+      | cons p1 p2 s_ s'_ s''_ k_ tree rest =>
+        cases tree with
+          | ss_seq1 p1 p2 s__ s'__ ih_finished =>
+            refine BigStep.bs_seq p1 p2 s s'_ s' ?_ ?_
+            have k_gt_zero : k_ > 0 := small_step_sequence_gt_zero rest
+            have zero_lt_k : 0 < k_ := by exact k_gt_zero
+            have one_less : 1 < 1 + k_ := by
+              rw [Nat.add_comm]
+              apply Nat.succ_lt_succ
+              exact zero_lt_k
+            exact ih 1 one_less p1 s s'_ (SmallStepSequence.single p1 s s'_ ih_finished)
+            have k_less : k_ < 1 + k_ := by
+              rw [Nat.add_comm]
+              exact Nat.lt_add_one k_
+            exact ih k_ k_less p2 s'_ s' rest
+          | ss_seq2 p1 p2 p3 s__ s'__ ih_unfinished =>
+            have ⟨k1_, k2_, inbetween, ⟨⟨step1, step2⟩, arith⟩⟩ := small_step_sequence_seperable (1 + k_) p1 p2 s s' small_step2
+            have k1_gt_zero : k1_ > 0 := small_step_sequence_gt_zero step1
+            have k2_gt_zero : k2_ > 0 := small_step_sequence_gt_zero step2
+            have k1_lt_1_plus_k_ : k1_ < 1 + k_ := by
+              rw [<- arith]
+              refine Nat.lt_add_of_pos_right ?_
+              exact k2_gt_zero
+            have k2_lt_1_plus_k_ : k2_ < 1 + k_ := by
+              rw [<- arith]
+              rw [Nat.add_comm]
+              refine Nat.lt_add_of_pos_right ?_
+              exact k1_gt_zero
+
+            have step1_ih := ih k1_ k1_lt_1_plus_k_ p1 s inbetween step1
+            have step2_ih := ih k2_ k2_lt_1_plus_k_ p2 inbetween s' step2
+            exact
+              BigStep.bs_seq p1 p2 s inbetween s' (ih k1_ k1_lt_1_plus_k_ p1 s inbetween step1)
+                step2_ih
+
+          | ss_if_true b_expr p2 p_else s eval =>
+            have k_less : k_ < 1 + k_ := by
+              rw [Nat.add_comm]
+              exact Nat.lt_add_one k_
+            refine BigStep.bs_if_true b_expr p2 p_else s s' eval ?subtree
+            exact ih k_ k_less p2 s s' rest
+
+          | ss_if_false b_expr pthen p2 s eval =>
+            have k_less : k_ < 1 + k_ := by
+              rw [Nat.add_comm]
+              exact Nat.lt_add_one k_
+            refine BigStep.bs_if_false b_expr pthen p2 s s' eval ?subtree2
+            exact ih k_ k_less p2 s s' rest
+
+          | ss_while b_expr pbody s =>
+            have k_less : k_ < 1 + k_ := by
+              rw [Nat.add_comm]
+              exact Nat.lt_add_one k_
+            have rest_tree := ih k_ k_less (IMPProgram.if b_expr (pbody.seq (IMPProgram.while b_expr pbody)) IMPProgram.skip) s s' rest
+            cases eval_bool: ((evalBoolExpr b_expr).run s).fst with
+              | true =>
+                let rest_tree2 := rest_tree
+                cases rest_tree with
+                  | bs_if_true b_expr pthen pelse s s' eval_bs body_tree =>
+                    have pure := IMPState.eval_bool_is_pure s b_expr
+                    conv at eval_bool =>
+                      unfold StateT.run
+                    rw [eval_bool] at pure
+                    cases body_tree with
+                      | bs_seq p1 p2 s s1 s2 body_step rest_step =>
+                        refine BigStep.bs_while_true b_expr pbody s ?inbetween s' pure ?body ?next_loop
+                        exact s1
+                        exact body_step
+                        exact rest_step
+                  | bs_if_false _ _ _ _ _ eval_bs =>
+                    have eval_bs := by
+                      exact congrArg Prod.fst eval_bs
+                    simp at eval_bs
+                    rw [eval_bool] at eval_bs
+                    contradiction
+              | false =>
+                cases rest_tree with
+                  | bs_if_true _ _ _ _ _ eval_bs =>
+                    have eval_bs := by
+                      exact congrArg Prod.fst eval_bs
+                    simp at eval_bs
+                    rw [eval_bool] at eval_bs
+                    contradiction
+                  | bs_if_false b_expr pthen pelse s s' eval subtree =>
+                    cases subtree with
+                    | bs_skip s_new => exact BigStep.bs_while_false b_expr pbody s eval
