LeanIMP/SmallStep.lean
@@ -1,17 +1,96 @@
 import LeanIMP.Basic
 import LeanIMP.SmallStepBasic
 
-theorem small_step_sequence_composeable {α: Type} [BEq α] {p1 p2: IMPProgram α} {s s' s'' : IMPState α} :
- SmallStepSequence p1 s s' ->
- SmallStepSequence p2 s' s'' ->
- SmallStepSequence (IMPProgram.seq p1 p2) s s'' :=
+theorem small_step_sequence_composeable {α: Type} [BEq α] {p1 p2: IMPProgram α} {s s' s'' : IMPState α} {k1 k2: Nat} :
+ SmallStepSequence p1 s s' k1 ->
+ SmallStepSequence p2 s' s'' k2 ->
+ SmallStepSequence (IMPProgram.seq p1 p2) s s'' (k1 + k2) :=
  by
   intros step1 step2
   induction step1 with
     | single p s s' tree1 =>
       have tree1_step := SmallStep.ss_seq1 p p2 s s' tree1
-      exact SmallStepSequence.cons (IMPProgram.seq p p2) p2 s s' s'' tree1_step step2
-    | cons p1 p2_cons s s' s''_cons next tail ih =>
+      exact SmallStepSequence.cons (IMPProgram.seq p p2) p2 s s' s'' k2 tree1_step step2
+    | cons p1 p2_cons s s' s''_cons k next tail ih =>
       have ih := ih step2
       have next_step := SmallStep.ss_seq2 p1 p2 p2_cons s s' next
-      exact SmallStepSequence.cons (IMPProgram.seq p1 p2) (IMPProgram.seq p2_cons p2) s s' s'' next_step ih
+      rw [Nat.add_assoc]
+      exact SmallStepSequence.cons (IMPProgram.seq p1 p2) (IMPProgram.seq p2_cons p2) s s' s'' (k+k2) next_step ih
+
+
+theorem small_step_sequence_gt_zero {α: Type} [BEq α] {p: IMPProgram α} {s s': IMPState α} {k: Nat}
+  (seq: SmallStepSequence p s s' k) : k > 0 := by
+    induction seq with
+      | single _ _ _ => trivial
+      | cons _ _ _ _ _ k _ _ ih => exact Nat.add_pos_right 1 ih
+
+
+-- https://github.com/leanprover/lean4/blob/ff6eb56f5c0ffff7b0c6b27add542e725767f37b/tests/playground/pge.lean
+theorem lt_or_eq_of_succ {i j:Nat} (lt : i < Nat.succ j) : i < j ∨ i = j :=
+  match lt with
+  | Nat.le.step m => Or.inl m
+  | Nat.le.refl => Or.inr rfl
+
+theorem strong_induction_on (p : Nat → Prop) (n:Nat)
+  (h:∀n, (∀ m, m < n → p m) → p n) : p n := by
+    suffices ∀n m, m < n → p m from this (Nat.succ n) n (Nat.lt_succ_self _)
+    intros n
+    induction n with
+    | zero =>
+      intros m h
+      contradiction
+    | succ i ind =>
+      intros m h1
+      cases lt_or_eq_of_succ h1 with
+      | inl is_lt =>
+        apply ind _ is_lt
+      | inr is_eq =>
+        apply h
+        rw [is_eq]
+        apply ind
+
+
+theorem small_step_sequence_seperable {α: Type} [BEq α] :
+  ∀k: Nat, ∀p1 p2: IMPProgram α, ∀s s'': IMPState α, SmallStepSequence (IMPProgram.seq p1 p2) s s'' k ->
+  ∃k1 k2: Nat, ∃s': IMPState α, And (And (SmallStepSequence p1 s s' k1) (SmallStepSequence p2 s' s'' k2)) (k1 + k2 = k) :=
+    by
+      intros k
+      refine strong_induction_on (fun x => (∀p1 p2: IMPProgram α, ∀s s'': IMPState α, (⟨p1.seq p2,s⟩ ->* [x] s'') -> ∃k1' k2': Nat, ∃s': IMPState α, And (And (SmallStepSequence p1 s s' k1') (SmallStepSequence p2 s' s'' k2')) (k1' + k2' = x))) k ?_
+      simp
+      intros n
+      intros ih
+      intros p1 p2
+      intros s s''
+      intros composed_sequence
+      cases composed_sequence with
+        | single tree =>
+          exists 1
+        | cons p1 p2_cons s s' s'' k1 step rest =>
+          cases step with
+            | ss_seq1 p1 p2 _ _ ih_finished =>
+              exists 1
+              exists k1
+              constructor
+              exists s'
+              exact And.intro (SmallStepSequence.single p1 s s' ih_finished) rest
+              simp
+            | ss_seq2 p1 p2 p3 s s' ih_unfinished =>
+              have k_less : k1 < 1 + k1 := by
+                rw [Nat.add_comm]
+                exact Nat.lt_add_one k1
+              have ⟨k1_, k2_, ⟨inbetween, ⟨step1, step2⟩⟩, arith⟩ := ih k1 k_less p3 p2 s' s'' rest
+              have a := SmallStepSequence.cons p1 p3 s s' inbetween k1_ ih_unfinished step1
+              exists (k1_+1)
+              exists k2_
+              constructor
+              exists inbetween
+              constructor
+              rw [Nat.add_comm]
+              exact a
+              exact step2
+              conv =>
+                arg 1
+                arg 1
+                rw [Nat.add_comm]
+              rw [Nat.add_assoc]
+              rw [arith]
